progs/verif_io.v
@@ -1,18 +1,6 @@
 Require Import VST.progs.io.
 Require Import VST.progs.io_specs.
 Require Import VST.floyd.proofauto.
-Require Import ITree.ITree.
-Require Import ITree.Eq.Eq.
-(*Import ITreeNotations.*)
-Notation "t1 >>= k2" := (ITree.bind t1 k2)
-  (at level 50, left associativity) : itree_scope.
-Notation "x <- t1 ;; t2" := (ITree.bind t1 (fun x => t2))
-  (at level 100, t1 at next level, right associativity) : itree_scope.
-Notation "t1 ;; t2" := (ITree.bind t1 (fun _ => t2))
-  (at level 100, right associativity) : itree_scope.
-Notation "' p <- t1 ;; t2" :=
-  (ITree.bind t1 (fun x_ => match x_ with p => t2 end))
-(at level 100, t1 at next level, p pattern, right associativity) : itree_scope.
 
 Instance CompSpecs : compspecs. make_compspecs prog. Defined.
 Definition Vprog : varspecs. mk_varspecs prog. Defined.
@@ -312,7 +300,7 @@ Lemma body_main: semax_body Vprog Gprog f_main main_spec.
 Proof.
   start_function.
   unfold main_pre_ext.
-  sep_apply (has_ext_ITREE(file_id := nat)).
+  sep_apply (has_ext_ITREE(E := @IO_event nat)).
   forward.
   unfold main_itree.
   rewrite <- !seq_assoc. (* Without this, forward_call gives a type error! *)
