progs/verif_printf.v
@@ -6,7 +6,8 @@ Definition Vprog : varspecs. mk_varspecs prog. Defined.
 Require Import VST.floyd.printf.
 Require Import ITree.Eq.Eq.
 
-Instance nat_id : FileId := { file_id := nat; stdout := 1%nat }.
+Instance nat_id : FileId := { file_id := nat; stdin := 0%nat; stdout := 1%nat }.
+Instance file_struct : FileStruct := {| FILEid := ___sFILE64; reent := __reent; f_stdin := __stdin; f_stdout := __stdout |}.
 
 Definition main_spec :=
  DECLARE _main
@@ -29,17 +30,18 @@ Qed.
 Lemma body_main: semax_body Vprog Gprog f_main main_spec.
 Proof.
 start_function.
-sep_apply (init_stdio gv __stdout).
+make_stdio.
 repeat do_string2bytes.
 repeat (sep_apply data_at_to_cstring; []).
-sep_apply (has_ext_ITREE(file_id := file_id)).
+sep_apply (has_ext_ITREE(E := @IO_event file_id)).
 forward_printf tt (write_list stdout (string2bytes "This is line 2.
 ")).
 { rewrite !sepcon_assoc; apply sepcon_derives; cancel.
   apply derives_refl. }
-forward_fprintf (gv __stdout) ((Ers, string2bytes "line", gv ___stringlit_2), (Int.repr 2, tt)) (stdout, Ret tt : @IO_itree file_id).
-{ rewrite sepcon_comm; apply sepcon_derives; cancel.
-  apply ITREE_impl.
-  rewrite bind_ret'; reflexivity. }
+forward_call.
+forward.
+forward_fprintf outp ((Ers, string2bytes "line", gv ___stringlit_2), (Int.repr 2, tt)) (stdout, Ret tt : @IO_itree (@IO_event file_id)).
+{ rewrite 3sepcon_assoc, sepcon_comm, sepcon_assoc; apply sepcon_derives; cancel.
+  rewrite bind_ret'; apply derives_refl. }
 forward.
 Qed.
